theories/Reflection2/PredMonadState.v
@@ -6,10 +6,12 @@ Require Export PredMonad.Reflection2.MonadState.
  *** Predicate Monads with State Effects
  ***)
 
-Class PredMonadState M PM St {OM: OTypeF1 M} {OPM: OTypeF1 PM} {OSt: OType St}
-      {MOps: @MonadOps M OM} {PMOps: @MonadOps PM OPM}
-      {PredOps: @PredMonadOps M PM OM OPM}
-      {MSOps: @MonadStateOps M OM St OSt} {PMSOps: @MonadStateOps PM OPM St OSt}
+Class PredMonadState M PM St {OM} {FOM: FindOTypeF1 M OM}
+      {OPM} {FOPM: FindOTypeF1 PM OPM} {OSt: OType St}
+      {MOps: @MonadOps M OM FOM} {PMOps: @MonadOps PM OPM FOPM}
+      {PredOps: @PredMonadOps M PM OM FOM OPM FOPM}
+      {MSOps: @MonadStateOps M OM FOM St OSt}
+      {PMSOps: @MonadStateOps PM OPM FOPM St OSt}
   : Prop :=
   {
     (* M and PM must form a predicate monad *)
